super clean

Cm/Pi/Infer.lean
@@ -337,18 +337,26 @@ def infer_eq.inject_future_infer'' : Expr :=
       (q' q' (quote apply))
         (:: (q' both) (::
           (q' q' both)
-          (:: (q' both) (::
-            (mk_both' 1 (::
+          (mk_both' 1 (::
+            (::
               (q' q' const)
-              Expr.id))
+              Expr.id)
           (q' q' infer.assert_well_typed_unsafe)))))))))
 
-
+def infer_eq.inject_future_infer''' : Expr :=
+  mk_both' 0 (mk_both' 1 (::
+    (q' q' both)
+    (::
+      (q' q' (quote apply))
+        (:: (q' q' both) (::
+            (:: (q' q' const) Expr.id)
+            (q' q' infer.assert_well_typed_unsafe))))))
 
 example : (quote (quote infer.assert_well_typed_unsafe)) = (q' q' infer.assert_well_typed_unsafe) := rfl
 
 example : infer_eq.inject_future_infer = infer_eq.inject_future_infer' := rfl
 example : infer_eq.inject_future_infer = infer_eq.inject_future_infer'' := rfl
+example : infer_eq.inject_future_infer = infer_eq.inject_future_infer''' := rfl
 
 
 /-
